more

thys/Substitution/Expression_Like_Birecursor.thy
@@ -2,11 +2,118 @@ theory Expression_Like_Birecursor
   imports Expression_Like_Sub
 begin
 
+locale Bimodel = Nominal Pperm "PVrs :: 'p \<Rightarrow> 'a :: var set" + Expression Eperm "EVrs :: 'e \<Rightarrow> 'a set" Ector
+  for Pperm PVrs Eperm EVrs Ector +
+  fixes  is_base :: "('a::var, 'a, 'e, 'e) G \<Rightarrow> bool"
+  and Ector_base :: "('a::var, 'a, 'e, 'e) G \<Rightarrow> 'p \<Rightarrow> 'e"
+  and Ector_step :: "('a::var, 'a, 'p \<Rightarrow> 'e, 'p \<Rightarrow> 'e) G \<Rightarrow> 'p \<Rightarrow> 'e"
+  assumes "\<exists>P. P is_base Ector_base Ector_step"
+
+locale Birecursor = Bimodel Pperm "PVrs :: 'p \<Rightarrow> 'a set" Eperm "EVrs :: 'e \<Rightarrow> 'a :: var set" Ector is_base Ector_base Ector_step
+  for Pperm PVrs Eperm EVrs Ector is_base Ector_base Ector_step +
+  assumes rec: "\<exists>!rec.
+      ((\<forall>u p. is_base u \<longrightarrow> GVrs2 u \<inter> PVrs p = {} \<longrightarrow> rec (Ector u) p = Ector_base u p) \<and>
+       (\<forall>u p. \<not> is_base u \<longrightarrow> GVrs2 u \<inter> PVrs p = {} \<longrightarrow> rec (Ector u) p = Ector_step (Gmap rec rec u) p) \<and>
+       (\<forall>e p \<sigma>. bij \<sigma> \<longrightarrow> |supp \<sigma>| <o |UNIV :: 'a set| \<longrightarrow> rec (Eperm \<sigma> e) p = Eperm \<sigma> (rec e (Pperm (inv \<sigma>) p))) \<and>
+       (\<forall>e p. EVrs (rec e p) \<subseteq> PVrs p \<union> EVrs e))"
+begin
+
+definition rec where
+  "rec = (THE rec. ((\<forall>u p. is_base u \<longrightarrow> GVrs2 u \<inter> PVrs p = {} \<longrightarrow> rec (Ector u) p = Ector_base u p) \<and>
+       (\<forall>u p. \<not> is_base u \<longrightarrow> GVrs2 u \<inter> PVrs p = {} \<longrightarrow> rec (Ector u) p = Ector_step (Gmap rec rec u) p) \<and>
+       (\<forall>e p \<sigma>. bij \<sigma> \<longrightarrow> |supp \<sigma>| <o |UNIV :: 'a set| \<longrightarrow> rec (Eperm \<sigma> e) p = Eperm \<sigma> (rec e (Pperm (inv \<sigma>) p))) \<and>
+       (\<forall>e p. EVrs (rec e p) \<subseteq> PVrs p \<union> EVrs e)))"
+
+lemma rec_base: "is_base u \<Longrightarrow> GVrs2 u \<inter> PVrs p = {} \<Longrightarrow> rec (Ector u) p = Ector_base u p"
+  using theI'[OF rec, THEN conjunct1] unfolding rec_def
+  by blast
+
+lemma rec_Ector: "\<not> is_base u \<Longrightarrow> GVrs2 u \<inter> PVrs p = {} \<Longrightarrow> rec (Ector u) p = Ector_step (Gmap rec rec u) p"
+  using theI'[OF rec, THEN conjunct2, THEN conjunct1] unfolding rec_def
+  by blast
+
+lemma rec_EPerm: "bij \<sigma> \<Longrightarrow> |supp \<sigma>| <o |UNIV :: 'a set| \<Longrightarrow> rec (Eperm \<sigma> e) p = Eperm \<sigma> (rec e (Pperm (inv \<sigma>) p))"
+  using theI'[OF rec, THEN conjunct2, THEN conjunct2, THEN conjunct1] unfolding rec_def
+  by blast
+
+lemma rec_EVrs: "EVrs (rec e p) \<subseteq> PVrs p \<union> EVrs e"
+  using theI'[OF rec, THEN conjunct2, THEN conjunct2, THEN conjunct2] unfolding rec_def
+  by blast
+
+end
+
 context Expression begin
 
-(*TODO provide definition and proof *)
+lemma permute_\<rho>:
+  "bij f \<Longrightarrow> |supp f| <o |UNIV :: 'a set| \<Longrightarrow> imsupp f \<inter> IImsupp' (Ector \<circ> \<eta>) EVrs \<rho> = {} \<Longrightarrow> Eperm f (\<rho> a) = \<rho> (f a)"
+  apply (cases "f a = a")
+   apply (cases "\<rho> a = Ector (\<eta> a)")
+    apply (simp add: Gren_def eta_natural Eperm_Ector)
+   apply simp
+   apply (rule Eperm_cong_id; simp?)
+  subgoal for a'
+    apply (subgoal_tac "a' \<in> IImsupp' (Ector \<circ> \<eta>) EVrs \<rho>")
+     apply (meson Int_emptyD not_in_imsupp_same)
+    apply (auto simp: IImsupp'_def IImsupp_def SSupp_def)
+    done
+  apply (cases "\<rho> a = Ector (\<eta> a)")
+   apply (simp add: Gren_def eta_natural Eperm_Ector)
+   apply (auto simp: IImsupp'_def IImsupp_def SSupp_def imsupp_def supp_def)
+  done
+
+lemma permute_\<rho>':
+  "bij f \<Longrightarrow> |supp f| <o |UNIV :: 'a set| \<Longrightarrow> imsupp f \<inter> IImsupp' (Ector \<circ> \<eta>') EVrs \<rho>' = {} \<Longrightarrow> Eperm f (\<rho>' a) = \<rho>' (f a)"
+  apply (cases "f a = a")
+   apply (cases "\<rho>' a = Ector (\<eta>' a)")
+    apply (simp add: Gren_def eta'_natural Eperm_Ector)
+   apply simp
+   apply (rule Eperm_cong_id; simp?)
+  subgoal for a'
+    apply (subgoal_tac "a' \<in> IImsupp' (Ector \<circ> \<eta>') EVrs \<rho>'")
+     apply (meson Int_emptyD not_in_imsupp_same)
+    apply (auto simp: IImsupp'_def IImsupp_def SSupp_def)
+    done
+  apply (cases "\<rho>' a = Ector (\<eta>' a)")
+   apply (simp add: Gren_def eta'_natural Eperm_Ector)
+   apply (auto simp: IImsupp'_def IImsupp_def SSupp_def imsupp_def supp_def)
+  done
+
+sublocale Esub: Bimodel where
+  Pperm = "\<lambda>\<sigma> (\<delta>, \<rho>, \<rho>'). (\<sigma> o \<delta> o inv \<sigma>, Eperm \<sigma> o \<rho> o inv \<sigma>, Eperm \<sigma> o \<rho>' o inv \<sigma>)" and
+  PVrs = "\<lambda>(\<delta>, \<rho>, \<rho>'). imsupp \<delta> \<union> IImsupp' (Ector \<circ> \<eta>) EVrs \<rho> \<union> IImsupp' (Ector \<circ> \<eta>') EVrs \<rho>'" and
+  Eperm = Eperm and
+  EVrs = EVrs and
+  Ector = Ector and
+  is_base = "\<lambda>u. \<exists>a. u = \<eta> a \<or> u = \<eta>' a" and
+  Ector_base = "\<lambda>u (\<delta>, \<rho>, \<rho>'). if (\<exists>a. u = \<eta> a) then \<rho> (SOME a. u = \<eta> a) else \<rho>' (SOME a. u = \<eta>' a)" and
+  Ector_step = "\<lambda>u (\<delta>, \<rho>, \<rho>'). Ector (Gmap (\<lambda>rec. rec (\<delta>, \<rho>, \<rho>')) (\<lambda>rec. rec (\<delta>, \<rho>, \<rho>')) u)"
+  apply standard
+  subgoal for \<sigma> \<tau>
+    by (auto simp: fun_eq_iff o_inv_distrib Eperm_comp[THEN fun_cong, simplified])
+  subgoal for \<sigma> p
+    apply (cases p)
+    apply (auto simp: fun_eq_iff)
+      apply (metis in_imsupp inv_simp1 inv_simp2 not_in_imsupp_same)
+     apply (metis (no_types, lifting) Int_emptyI bij_id_imsupp inv_simp2 permute_\<rho>)
+    apply (metis (no_types, lifting) Int_emptyI bij_id_imsupp inv_simp2 permute_\<rho>')
+    done
+  subgoal
+    sorry
+  done
+
+sublocale rec: Birecursor
+  apply standard
+
+end
+
+context Birecursor begin
+
+term Esub.rec
+
 interpretation Substitution undefined
   apply standard
   sorry
+
+end
 
 end
